rsp_new.fst
@@ -1,0 +1,366 @@
+module Rsp_New
+
+open FStar.Calc
+open FStar.Tactics
+
+open Common
+open IOStHist
+open M4
+open Minterop
+
+type set_of_traces (a:Type) = events_trace * a -> Type0
+
+val included_in : (#a:Type) -> (#b:Type) -> (a -> b) -> set_of_traces a -> set_of_traces b -> Type0
+let included_in rel s1 s2 = forall t r. s1 (t, r) ==>  s2 (t, rel r)
+
+let rec behavior #a
+  (m : io a) : set_of_traces (maybe a) =
+  match m with
+  | Return x -> fun t -> t == ([], Inl x)
+  | Throw err -> fun t -> t == ([], Inr err)
+  | Cont t -> begin
+    match t with
+    | Call cmd args fnc -> (fun (t', r') -> 
+      (exists (res:resm cmd) t. (
+         FStar.WellFounded.axiom1 fnc res;
+         (behavior (fnc res) (t,r')) /\
+         t' == (convert_call_to_event cmd args res)::t)))
+  end
+
+let empty_set (#a:Type) () : set_of_traces a = fun (t,r) -> t == []
+
+let id #a (x:a) = x
+
+let export_in_empty_set (a:Type) {| d:exportable a |} () :
+  Lemma (forall (x:a).
+    behavior (io_return _ (export x)) 
+      `included_in id` 
+    (empty_set ())) = ()
+      
+let beh_shift_trace
+  #a
+  (cmd : io_cmds)
+  (argz : args cmd)
+  (rez : resm cmd)
+  (fnc : resm cmd -> io a)
+  (t:events_trace)
+  (r:maybe a) :
+  Lemma 
+    (requires (behavior (Cont (Call cmd argz fnc)) ((convert_call_to_event cmd argz rez :: t), r)))
+    (ensures (behavior (fnc rez) (t, r))) = () 
+
+let beh_extend_trace 
+  #a
+  (cmd : io_cmds)
+  (argz : args cmd)
+  (rez : resm cmd)
+  (fnc : resm cmd -> io a)
+  (t:events_trace)
+  (r:maybe a) :
+  Lemma
+    (requires (behavior (fnc rez) (t, r)))
+    (ensures (behavior (Cont (Call cmd argz fnc)) ((convert_call_to_event cmd argz rez) :: t, r))) by (compute ()) = ()
+
+let beh_extend_trace_in_bind 
+  #a #b
+  (cmd : io_cmds)
+  (argz : args cmd)
+  (rez : resm cmd)
+  (fnc : resm cmd -> io a)
+  (k : a -> io b)
+  (t:events_trace)
+  (r:maybe b) :
+  Lemma
+    (requires (behavior (io_bind a b (fnc rez) k) (t, r))) 
+    (ensures (behavior (io_bind a b (Cont (Call cmd argz fnc)) k) ((convert_call_to_event cmd argz rez) :: t, r))) =
+    calc (==) {
+      io_bind a b (Cont (Call cmd argz fnc)) k;
+      == {}
+      sys_bind io_cmds io_cmd_sig a b (Cont (Call cmd argz fnc)) k;
+      == { admit () }
+      Cont (sysf_fmap (fun fnci -> 
+        sys_bind io_cmds io_cmd_sig a b fnci k) (Call cmd argz fnc));
+      == { _ by (unfold_def(`sysf_fmap); norm [iota]; unfold_def(`io_bind)) }
+      Cont (Call cmd argz (fun rez -> 
+        io_bind a b (fnc rez) k));
+    };
+    beh_extend_trace cmd argz rez (fun rez -> io_bind a b (fnc rez) k) t r;
+    assert (behavior (Cont (Call cmd argz (fun rez -> 
+        io_bind a b (fnc rez) k))) ((convert_call_to_event cmd argz rez) :: t, r)) by (
+          unfold_def (`convert_call_to_event); assumption (); dump "H")
+
+let extract_result (cmd:io_cmds) (event:io_event) : Pure (resm cmd)
+  (requires ((cmd == Openfile ==>  EOpenfile? event) \/
+      (cmd == Read ==> ERead? event) \/
+      (cmd == Close ==> EClose? event)))
+  (ensures (fun r -> True)) = 
+  admit ();
+  match cmd with 
+  | Openfile -> EOpenfile?.r event 
+  | Read -> ERead?.r event 
+  | Close -> EClose?.r event 
+    
+let rec beh_bind_inl
+  #a #b
+  (m : io a)
+  (k : a -> io b) 
+  (r1:a) 
+  (t1 t2 : events_trace)
+  (r2:maybe b) :
+  Lemma 
+    (requires (behavior m (t1, (Inl r1)) /\ behavior (k r1) (t2, r2)))
+    (ensures (behavior (io_bind _ _ m k) (t1 @ t2, r2))) =
+  match m with
+  | Return x -> ()
+  | Throw err -> ()
+  | Cont (Call cmd argz fnc) -> begin
+    let (ht1 :: tt1) = t1 in
+    let rez : resm cmd = extract_result cmd ht1 in
+    FStar.WellFounded.axiom1 fnc rez;
+    beh_shift_trace cmd argz rez fnc tt1 (Inl r1);
+    beh_bind_inl (fnc rez) k r1 tt1 t2 r2;
+    beh_extend_trace_in_bind cmd argz rez fnc k (tt1@t2) r2
+  end
+  
+let rec beh_bind_inr
+  #a #b
+  (m : io a)
+  (k : a -> io b)
+  (r1:exn)
+  (t1 : events_trace) :
+  Lemma 
+    (requires (behavior m (t1, (Inr r1))))
+    (ensures (behavior (io_bind _ _ m k) (t1, (Inr r1)))) =
+  match m with
+  | Throw err -> ()
+  | Cont (Call cmd argz fnc) -> begin
+    let (ht1 :: tt1) = t1 in
+    let rez : resm cmd = extract_result cmd ht1 in
+    FStar.WellFounded.axiom1 fnc rez;
+    beh_shift_trace cmd argz rez fnc tt1 (Inr r1);
+    beh_bind_inr (fnc rez) k r1 tt1;
+    beh_extend_trace_in_bind cmd argz rez fnc k (tt1) (Inr r1)
+  end
+
+let beh_bind_0 
+  #a #b
+  (m : io a)
+  (k : a -> io b) 
+  (r1:maybe a) :
+  Lemma (forall t1.
+    behavior m (t1, r1) ==>
+      (Inr? r1 ==>  behavior (io_bind _ _ m k) (t1, (Inr (Inr?.v r1)))) /\
+      (Inl? r1 ==>  (forall t2 r2. (behavior (k (Inl?.v r1)) (t2, r2) ==>  
+                     behavior (io_bind _ _ m k) (t1 @ t2, r2))))) =
+  if (Inr? r1) then (
+    Classical.forall_intro (
+      Classical.move_requires (beh_bind_inr m k (Inr?.v r1)))
+  ) else (
+    Classical.forall_intro_3 (
+      Classical.move_requires_3 (beh_bind_inl m k (Inl?.v r1)))
+  )
+
+
+let beh_bind
+  #a #b
+  (m : io a)
+  (k : a -> io b) :
+  Lemma (forall (r1:maybe a) t1.
+    behavior m (t1, r1) ==>
+      (Inr? r1 ==>  behavior (io_bind _ _ m k) (t1, (Inr (Inr?.v r1)))) /\
+      (Inl? r1 ==>  (forall t2 r2. behavior (k (Inl?.v r1)) (t2, r2) ==>  
+                              behavior (io_bind _ _ m k) (t1 @ t2, r2)))) =
+  Classical.forall_intro (beh_bind_0 m k)
+
+unfold let oal #a #b (f:a -> b) (x:maybe a) : maybe b =
+  match x with
+  | Inl x -> Inl (f x)
+  | Inr err -> Inr err
+ 
+let beh_bind_tot_0
+  #a #b
+  (f:io a)
+  (g:a -> Tot b)
+  (r:maybe a)
+  (t:events_trace) :
+  Lemma 
+    (requires (behavior f (t, r)))
+    (ensures (behavior (io_bind a b f (fun x -> io_return _ (g x)))) (t, (oal g r))) =
+ 
+  assert (forall (x:a). behavior (io_return _ (g x)) `included_in id` empty_set ());
+  beh_bind f (fun x -> io_return _ (g x));
+  if (Inr? r) then admit ()
+  else admit ()
+  
+let beh_bind_tot
+  #a #b
+  (f:io a)
+  (g:a -> Tot b) :
+  Lemma 
+    (forall r t. behavior f (t, r) ==> 
+      (behavior (io_bind a b f (fun x -> io_return _ (g x)))) (t, (oal g r))) =
+  Classical.forall_intro_2 (Classical.move_requires_2 (beh_bind_tot_0 f g))
+
+let beh_included_bind_tot
+  #a #b
+  (f:io a) 
+  (g:a -> Tot b):
+  Lemma
+    (included_in (oal g)
+      (behavior f)
+      (behavior (io_bind a b f (fun x -> io_return _ (g x))))) = 
+  beh_bind_tot #a #b f g;
+  ()
+
+let iost_to_io #t2 (tree : io (events_trace * t2)) : io t2 =
+  match tree with
+  | Return (s1, r) -> Return r
+  | Throw r -> Throw r
+  | Cont (Call cmd argz fnc) ->
+    io_bind (events_trace * t2) t2
+      (Cont (Call cmd argz fnc))
+      (fun (_, r) -> io_return _ r)
+
+let behavior_iost_to_io () : 
+  Lemma (forall (a:Type) (tree:io (events_trace * a)). 
+    behavior (iost_to_io tree) `included_in` behavior tree) = admit ()
+
+
+
+unfold let ref #a (x : io a) : M4.irepr a (fun p -> forall res. p res) = (fun _ -> x)
+
+let _export_IOStHist_lemma #t1 #t2
+  {| d1:importable t1 |}
+  {| d2:exportable t2 |}
+  (pre : t1 -> events_trace -> Type0)
+  {| checkable2 pre |}
+  (post : t1 -> events_trace -> maybe (events_trace * t2) -> events_trace -> Type0)
+  (f:(x:t1 -> IOStHist t2 (pre x) (post x))) 
+  (x':d1.itype) : 
+  Lemma (match import x' with
+    | Some x -> (
+        let ef : d1.itype -> M4 d2.etype = _export_IOStHist_arrow_spec pre post f in
+        let res' = reify (ef x') (fun _ -> True) in
+
+        let f' = reify (f x) (post x []) in
+        check2 #t1 #events_trace #pre x [] ==>  behavior res' `included_in` behavior (f' []))
+        // TODO: prove that behavior of res is empty trace if check2 fails?
+    | None -> 
+       // TODO: prove that behavior of res is the empty trace if import fails?
+           True)=
+
+  match import x' with
+  | Some x -> begin
+    if (check2 #t1 #events_trace #pre x []) then (
+        let ef : d1.itype -> M4 d2.etype = _export_IOStHist_arrow_spec pre post f in
+        calc (included_in) {
+            behavior (reify (ef x') (fun _ -> True));
+            `included_in` {}
+            behavior (reify ((_export_IOStHist_arrow_spec pre post f <: (d1.itype -> M4 d2.etype)) x') (fun _ -> True));
+            `included_in` { _ by (unfold_def(`_export_IOStHist_arrow_spec); norm [delta]) }
+            behavior (reify (
+              (export (M4wp?.reflect (ref (iost_to_io (reify (f x) (post x []) []))) <: M4wp t2 (fun p -> forall res. p res)) <: d2.etype)) (fun _ -> True));
+            == { admit () } // unfold reify
+            // Cezar: is the 3rd argument correct? I suppose it should pre and post
+            behavior (M4.ibind t2 d2.etype (fun p -> forall res. p res) (fun x -> m4_return_wp (d2.etype) (export x))
+                (reify (M4wp?.reflect (ref (iost_to_io (reify (f x) (post x []) []))) <: M4wp t2 (fun p -> forall res. p res)))
+                (fun x -> lift_pure_m4wp d2.etype (fun p -> p (export x)) (fun _ -> export x)) (fun _ -> True));
+            `included_in` { _ by (unfold_def (`ibind); dump "H"); admit () }
+            behavior (M4.ibind t2 d2.etype (fun p -> forall res. p res) (fun x -> m4_return_wp (d2.etype) (export x))
+                (ref (iost_to_io (reify (f x) (post x []) [])))
+                (fun x -> lift_pure_m4wp d2.etype (fun p -> p (export x)) (fun _ -> export x)) (fun _ -> True));
+        //     `included_in` { test  (ref (iost_to_io (reify (f x) (post x []) []))) }
+        //     // `included_in` { _ by (norm [iota]; dump "h") }
+            == { admit () }
+            behavior (iost_to_io (reify (f x) (post x []) []));
+            `included_in` { behavior_iost_to_io () }
+            behavior (reify (f x) (post x []) []);
+        }
+    ) else ()
+  end
+  | None -> ()
+
+
+let export_IOStHist_lemma 
+  #t1 {| d1:importable t1 |} 
+  #t2 {| d2:exportable t2 |}
+  (pre : t1 -> events_trace -> Type0) {| checkable2 pre |}
+  (post : t1 -> events_trace -> maybe (events_trace * t2) -> events_trace -> Type0)
+  (f:(x:t1 -> IOStHist t2 (pre x) (post x))) : 
+  Lemma (forall (x':d1.itype). (
+    match import x' with
+    | Some x -> (
+        let ef : d1.itype -> M4 d2.etype = export f in
+        let res' = reify (ef x') (fun _ -> True) in
+
+        let f' = reify (f x) (post x []) in
+
+        check2 #t1 #events_trace #pre x [] == true ==>  behavior res' `included_in` behavior (f' []))
+    | None -> True)) =
+  Classical.forall_intro (_export_IOStHist_lemma #t1 #t2 pre post f)
+
+
+let export_GIO_lemma 
+  #t1 {| d1:importable t1 |} 
+  #t2 {| d2:exportable t2 |}
+  (pi:check_type)
+  (f:(x:t1 -> GIO t2 pi)) : 
+  Lemma (forall (x':d1.itype). (
+    match import x' with
+    | Some x -> (
+        let ef : d1.itype -> M4 d2.etype = export f in
+        let res' = reify (ef x') (fun _ -> True) in
+
+        let f' = reify (f x) (gio_post pi []) in
+
+        check2 #t1 #events_trace #(fun _ -> gio_pre pi) x [] == true ==>  behavior res' `included_in` behavior (f' []))
+    | None -> True)) =
+  Classical.forall_intro (_export_IOStHist_lemma (fun _ -> gio_pre pi) (fun _ -> gio_post pi) f)
+
+let export_GIO_lemma' 
+  #t1 {| d1:importable t1 |} 
+  #t2 {| d2:exportable t2 |}
+  (pi:check_type)
+  (f:(x:t1 -> GIO t2 pi)) : 
+  Lemma (forall (x':d1.itype). (
+    match import x' with
+    | Some x -> (
+        let ef : d1.itype -> M4 d2.etype = _export_IOStHist_arrow_spec (fun _ -> gio_pre pi) (fun _ -> gio_post pi) f in
+        let res' = reify (ef x') (fun _ -> True) in
+
+        let f' = reify (f x) (gio_post pi []) in
+
+        check2 #t1 #events_trace #(fun _ -> gio_pre pi) x [] == true ==>  behavior res' `included_in` behavior (f' []))
+    | None -> True)) =
+  Classical.forall_intro (_export_IOStHist_lemma (fun _ -> gio_pre pi) (fun _ -> gio_post pi) f)
+
+let rsp_left 
+  (a : Type) {| d1:exportable a |}
+  (b : Type) {| d2:ml b |}
+  (c : Type) {| d3:exportable c |}
+  (pi : check_type)
+  (p : ((ct:(a -> GIO b pi)) -> GIO c pi))
+  (ct : (d1.etype -> M4 b)) :
+  Lemma (forall (pi_as_set:set_of_traces).
+    match import ct with
+    | Some (ct' : (pi:check_type) -> a -> GIO b pi) -> 
+        let pct : unit -> GIO c pi = fun _ -> p (ct' pi) in
+        let pct' : unit -> M4 d3.etype = _export_IOStHist_arrow_spec (fun _ -> gio_pre pi) (fun _ -> gio_post pi) pct in
+        behavior (reify (pct ()) (gio_post pi []) []) `included_in` pi_as_set ==> 
+        behavior (reify (pct' ()) (fun _ -> True)) `included_in` pi_as_set
+    | None -> False) // by (explode (); bump_nth 10; explode (); dump "h")
+  = 
+  match import ct with
+  | Some (ct' : (pi:check_type) -> a -> GIO b pi) -> 
+      let pct : unit -> GIO c pi = fun _ -> p (ct' pi) in
+      export_GIO_lemma pi pct;
+      let pct' : unit -> M4 d3.etype = _export_IOStHist_arrow_spec (fun _ -> gio_pre pi) (fun _ -> gio_post pi) pct in
+      export_GIO_lemma' pi pct;
+      calc (included_in) {
+        behavior (reify (pct' ()) (fun _ -> True));
+        `included_in` { _ by (dump "h") }
+        behavior (reify (pct ()) (gio_post pi []) []);
+        `included_in` {}
+        behavior (reify (p (ct' pi)) (gio_post pi []) []);
+      }
+  | None -> ()
